examples/unit-tests/bug44.fst
@@ -1,0 +1,11 @@
+module Bug44
+
+type nat =
+  | O : nat
+  | S : nat -> nat
+
+val lemma : n:nat -> Fact unit (ensures 0 < 42)
+let lemma n =
+  match n with
+  | O -> admit()
+  | S n' -> assert(False); admit()
